update LoVe09 Note

lean/LoVe/LoVe09_OperationalSemantics_Note.lean
@@ -46,14 +46,106 @@ def sillyLoop : Stmt :=
 /- ## 9.3 Big-Step Semantics -/
 
 /-
+(x := x + y; y := 0, [x ↦ 3 , y ↦ 5]) ⟹ [x ↦ 8, y ↦ 0]
+-/
+
+/-
 
 ---------------- SKIP
- (skip, s) => s
+ (skip, s) ⟹ s
 
 ---------------------------- ASSIGN
- (x := a, s) => s[x ↦ a s]
+ (x := a, s) ⟹ s[x ↦ a s]
 
+ (S, s) ⟹ t  (T, t) ⟹ u
+--------------------------- SEQ
+      (S; T, s) ⟹ u
 
+ (S, s) ⟹ t
+------------------------------- IF-TRUE if b s is true
+ (if b then S else T, s) ⟹ t
+
+ (T, s) ⟹ t
+------------------------------- IF-TRUE if b s is false
+ (if b then S else T, s) ⟹ t
+
+ (S, s) ⟹ t   (while b do S, t) ⟹ u
+--------------------------------------- WHILE-TRUE if b s is true
+ (while b do S, s) ⟹ u
+
+--------------------------- WHILE-FALSE if b s is false
+ (while b do S, s) ⟹ s
+
+where,
+  s[x ↦ n] = (fun v ↦ if v = x then n else s v)
 
 -/
+
+/-
+----------------------- ASSIGN  ------------------- ASSIGN
+ (x := x + y, s) ⟹ t            (y := 0, t) => u
+---------------------------------------------------- SEQ
+ (x := x + y; y := 0, s) ⟹ u
+-/
+
+inductive BigStep : Stmt × State → State → Prop where
+  | skip (s) :
+    BigStep (Stmt.skip, s) s
+  | assign (x a s) :
+    BigStep (Stmt.assign x a, s) (s[x ↦ a s])
+  | seq (S T s t u) (hS : BigStep (S, s) t) (hT : BigStep (T, t) u) :
+    BigStep (S; T, s) u
+  | if_true (B S T s t) (hcond : B s) (hbody : BigStep (S, s) t) :
+    BigStep (Stmt.ifThenElse B S T, s) t
+  | if_false (B S T s t) (hcond : ¬ B s) (hbody : BigStep (T, s) t) :
+    BigStep (Stmt.ifThenElse B S T, s) t
+  | while_true (B S s t u) (hcond : B s)
+    (hbody : BigStep (S, s) t) (hrest : BigStep (Stmt.whileDo B S, t) u) :
+    BigStep (Stmt.whileDo B S, s) u
+  | while_false (B S s) (hcond : ¬ B s) :
+    BigStep (Stmt.whileDo B S, s) s
+
+infix:110 " ⟹ " => BigStep
+
+theorem sillyLoop_from_1_BigStep :
+  (sillyLoop, (fun _ ↦ 0)["x" ↦ 1]) ⟹ (fun _ ↦ 0) := by
+  rw [sillyLoop]
+  apply BigStep.while_true
+  . simp
+  . apply BigStep.seq
+    . apply BigStep.skip
+    . apply BigStep.assign
+  . simp
+    apply BigStep.while_false
+    . simp
+
+/- ## 9.4 Properties of the Big-Step Semantics -/
+
+theorem BigStep_deterministic {Ss l r} (hl : Ss ⟹ l) (hr : Ss ⟹ r) :
+  l = r := by
+  induction hl generalizing r with
+  | skip s =>
+    cases hr with
+    | skip => rfl
+  | assign x a s =>
+    cases hr with
+    | assign => rfl
+  | seq S T s t u hS hT ihS ihT =>
+    cases hr with
+    | seq _ _ _ t' _ hS' hT' =>
+      apply ihS at hS'
+      rw [← hS'] at hT'
+      apply ihT at hT'
+      exact hT'
+  | if_true B S T s t hc hb ihb =>
+    cases hr with
+    | if_true _ _ _ _ _ hc' hb' =>
+      apply ihb hb'
+    | if_false _ _ _ _ _ hc' hb' =>
+      contradiction
+  | if_false B S T s t hc hb ih => sorry
+  | while_true B S s t u hc hb hrest ihb ihrest  => sorry
+  | while_false B S s hcond => sorry
+
+
 end LoVe
